clightplus/compiler_proof/ClightPlus2LBProof.v
@@ -2,22 +2,22 @@ From compcert Require Import Behaviors Lowerbound Compiler Complements.
 
 Set Implicit Arguments.
 
-Theorem transf_clight2_program_preservation_lbd
+Theorem transf_clight_program_preservation_lbd
     p tp
-    (T: transf_clight2_program p = Errors.OK tp) :
-  improves (Clight.semantics2 p) (Lowerbound.semantics tp).
+    (T: transf_clight_program p = Errors.OK tp) :
+  improves (Clight.semantics1 p) (Lowerbound.semantics tp).
 Proof.
-  apply Complements.transf_clight2_program_preservation_lbd.
-  apply transf_clight2_program_match. eauto.
+  apply Complements.transf_clight_program_preservation_lbd.
+  apply transf_clight_program_match. eauto.
 Qed.
 
-Theorem transf_clight2_program_via_SSA_preservation_lbd
+Theorem transf_clight_program_via_SSA_preservation_lbd
     p tp
-    (T: transf_clight2_program_via_SSA p = Errors.OK tp) :
-  improves (Clight.semantics2 p) (Lowerbound.semantics tp).
+    (T: transf_clight_program_via_SSA p = Errors.OK tp) :
+  improves (Clight.semantics1 p) (Lowerbound.semantics tp).
 Proof.
-  apply transf_clight2_program_preservation_ssa_lbd.
-  apply transf_clight2_program_via_SSA_match. eauto.
+  apply transf_clight_program_preservation_ssa_lbd.
+  apply transf_clight_program_via_SSA_match. eauto.
 Qed.
 
 Require Import Skeleton ModSem.
@@ -31,15 +31,15 @@ Theorem compile_behavior_improves_lbd
     (mn: string) (md: Mod.t) (sk_mem: Sk.t)
     (COMP: compile clight_prog mn = Errors.OK md)
     (MEMSKEL: mem_skel clight_prog = Errors.OK sk_mem)
-    (COMP': transf_clight2_program clight_prog = Errors.OK asm)
+    (COMP': transf_clight_program clight_prog = Errors.OK asm)
 :
     (improves2_program (clightp_sem sk_mem md) (Lowerbound.semantics asm)).
 Proof.
   eapply improves2_program_observe_trans.
   eapply single_compile_program_improves; eauto.
-  eapply transf_clight2_program_preservation_lbd in COMP'.
+  eapply transf_clight_program_preservation_lbd in COMP'.
   unfold Complements.improves in *. i. hexploit COMP'; eauto.
-  i. des. hexploit semantics2to3; eauto. i. des.
+  i. des. hexploit semantics1to3; eauto. i. des.
   esplits; eauto. eapply observation_improves_trans; eauto.
 Qed.
 
@@ -48,14 +48,14 @@ Theorem compile_behavior_improves_via_SSA_lbd
     (mn: string) (md: Mod.t) (sk_mem: Sk.t)
     (COMP: compile clight_prog mn = Errors.OK md)
     (MEMSKEL: mem_skel clight_prog = Errors.OK sk_mem)
-    (COMP': transf_clight2_program_via_SSA clight_prog = Errors.OK asm)
+    (COMP': transf_clight_program_via_SSA clight_prog = Errors.OK asm)
 :
     (improves2_program (clightp_sem sk_mem md) (Lowerbound.semantics asm)).
 Proof.
   eapply improves2_program_observe_trans.
   eapply single_compile_program_improves; eauto.
-  eapply transf_clight2_program_via_SSA_preservation_lbd in COMP'.
+  eapply transf_clight_program_via_SSA_preservation_lbd in COMP'.
   unfold Complements.improves in *. i. hexploit COMP'; eauto.
-  i. des. hexploit semantics2to3; eauto. i. des.
+  i. des. hexploit semantics1to3; eauto. i. des.
   esplits; eauto. eapply observation_improves_trans; eauto.
 Qed.
